fix proof

theories/util/basic.v
@@ -19,4 +19,4 @@ Lemma surjective_pairing_fun {A B C} (f: A → B * C) :
   f = (pair ∘ (fst ∘ f) ⊛ (snd ∘ f)).
 Proof. extensionality x. by rewrite /s_comb /compose -surjective_pairing. Qed.
 
-Definition pairmap {A B A' B'} (f: A → A') (g: B → B') xy := (f xy.1, g xy.2).
+Definition pair_map {A B A' B'} (f: A → A') (g: B → B') xy := (f xy.1, g xy.2).
