theories/typing/type.v
@@ -1,8 +1,4 @@
 From iris.algebra Require Import numbers list.
-From iris.algebra Require Import numbers list.
-From iris.algebra Require Import numbers list.
-From iris.algebra Require Import numbers list.
-From iris.algebra Require Import numbers list.
 From iris.base_logic Require Export na_invariants.
 From lrust.util Require Import basic types.
 From lrust.prophecy Require Export prophecy.
